examples/compute/src/bir_evalScript.sml
@@ -67,9 +67,9 @@ Theorem bir_eval_exp_update_env_den:
     !env var vimm. bir_eval_exp (bir_env_update env var vimm) (BExp_Den var) vimm
 Proof
     Cases_on `var` >>
-    rw [Once bir_eval_exp_cases, bir_env_update_def, bir_env_lookup_rel_cases] >>
+    rw [Once bir_eval_exp_cases, bir_env_update_def, bir_env_lookup_rel_def] >>
     qexists_tac `s` >>
-    rw [Once bir_eval_exp_cases, bir_env_update_def, bir_env_lookup_rel_cases]
+    rw [Once bir_eval_exp_cases, bir_env_update_def, bir_env_lookup_rel_def]
 QED
 
 
@@ -78,9 +78,9 @@ Theorem bir_eval_exp_empty_env_add:
         (BExp_BinExp BIExp_Plus (BExp_Const (Imm64 imm1)) (BExp_Const (Imm64 imm2)))
         (BVal_Imm (Imm64 (imm1 + imm2)))
 Proof
-    rw [Ntimes bir_eval_exp_cases 3, bir_eval_binexp_cases, 
+    rw [Ntimes bir_eval_exp_cases 3, bir_eval_binexp_def, 
         bir_eval_binexp_imm_cases, bir_binexp_get_oper_def] >>
-    rw [Once bir_eval_exp_cases, bir_eval_binexp_cases]
+    rw [Once bir_eval_exp_cases, bir_eval_binexp_def, bir_eval_binexp_imm_cases, bir_binexp_get_oper_def]
 QED
 
 
